---
output:
  html_document:
    theme: 'readable'
---

# Very Brief Matrix Differentiation
 
$$\begin{aligned} 
 \frac{d \boldsymbol a^T \boldsymbol x}{d \boldsymbol x} = \frac{d \boldsymbol  x ^T \boldsymbol a}{d \boldsymbol x} &= \boldsymbol a^T\\
 \frac{d \boldsymbol x^T \boldsymbol x}{d \boldsymbol x}&= 2 \boldsymbol x^T \\
 \frac{d (\boldsymbol x^T \boldsymbol a)^2}{d \boldsymbol x}&= 2 \boldsymbol x^T\\
 \frac{d \boldsymbol {Ax}}{d \boldsymbol x} &= \boldsymbol A \\
 \frac{d \boldsymbol {x}^T \boldsymbol A}{d \boldsymbol x} &= \boldsymbol A^T\\
 \frac{d \boldsymbol {x}^T \boldsymbol {Ax}}{d \boldsymbol x} &= \boldsymbol x^T ( \boldsymbol A + \boldsymbol A^T )
\end{aligned}$$

